Logic: Avoid UB around `const`
Also,

- Support `mutable` fields
- Some theory for `decompose_type`

Co-authored-by: Gregory Malecha <gregory@bedrocksystems.com>
Co-authored-by: Paolo G. Giarrusso <paolo@bedrocksystems.com>
Co-authored-by: David Swasey <david@bedrocksystems.com>

tests/const/cast.cpp
@@ -1,0 +1,49 @@
+
+void foo (int * const x) {
+
+  int * i = x;
+
+  int const * j = x;
+
+  int * const k = x;
+
+  int const * const l = x;
+
+  i = i;
+  //i = j; discards qualifiers
+  i = k;
+  //i = l; discards qualifiers
+
+  j = i;
+  j = j;
+  j = k;
+  j = l;
+
+
+  *i = *i;
+  *i = *j;
+  *i = *k;
+  *i = *l;
+
+  *k = *i;
+  *k = *j;
+  *k = *k;
+  *k = *l;
+}
+
+void
+bar() {
+
+  int x{0};
+
+  foo(&x);
+
+}
+
+
+int foo1(int const * p) { return *p; }
+
+void bar1() {
+  int x{0};
+  foo1(&x);
+}
