tests/const/const.cpp
@@ -1,0 +1,33 @@
+struct C {
+  const   int x{0};
+  mutable int y{0};
+  int         z{0};
+};
+struct D {
+          C c;
+  const   C cc;
+  mutable C mc;
+};
+
+void f() {
+        D d{};
+  const D cd{};
+
+  d.c.y = 1;
+  d.c.z = 1;
+  d.cc.y = 1;
+  d.mc.y = 1;
+  d.mc.z = 1;
+  
+  cd.c.y = 1;
+  cd.cc.y = 1;
+  cd.mc.y = 1;
+  cd.mc.z = 1;
+}
+
+/*
+void illegal() {
+  D d{};
+  d.c.x = 1; // UB
+}
+*/
