theories/lang/cpp/logic/func.v
@@ -9,8 +9,9 @@ Require Import bedrock.lang.bi.errors.
 Require Import bedrock.lang.cpp.logic.entailsN.
 Require Import bedrock.lang.cpp.ast.
 Require Import bedrock.lang.cpp.semantics.
+
 From bedrock.lang.cpp.logic Require Import
-  pred path_pred heap_pred wp builtins cptr
+  pred path_pred heap_pred wp builtins cptr const
   layout initializers destroy.
 
 #[local] Set Printing Coercions.
@@ -42,7 +43,7 @@ Section with_cpp.
      TODO replace this with a version that is built by well-founded recursion.
    *)
   #[local]
-  Fixpoint identitiesR' (f : nat) (include_base : bool) (cls : globname) (path : list globname) (q : Qp) : Rep :=
+  Fixpoint identitiesR' (f : nat) (include_base : bool) (cls : globname) (path : list globname) (q : cQp.t) : Rep :=
     match f with
     | 0 => False
     | S f =>
@@ -77,7 +78,7 @@ Section with_cpp.
       _base "::C" "::B" |-> identityR true "::B" ["::C"] q
       ]]
    *)
-  Definition identitiesR : bool -> globname -> list globname -> Qp -> Rep :=
+  Definition identitiesR : bool -> globname -> list globname -> cQp.t -> Rep :=
     let size := avl.IM.cardinal resolve.(genv_tu).(globals) in
     (* ^ the number of global entries is an upper bound on the height of the
        derivation tree.
@@ -89,8 +90,8 @@ Section with_cpp.
       for "this".
    *)
   Definition wp_init_identity (cls : globname) (Q : mpred) : Rep :=
-    identitiesR false cls [] 1 **
-    (identitiesR true cls [cls] 1 -* pureR Q).
+    identitiesR false cls [] (cQp.mut 1) **
+    (identitiesR true cls [cls] (cQp.mut 1) -* pureR Q).
 
   Theorem wp_init_identity_frame cls Q Q' :
     pureR (Q' -* Q) |-- wp_init_identity cls Q' -* wp_init_identity cls Q.
@@ -105,8 +106,8 @@ Section with_cpp.
       classes to remove [cls] as the most derived class.
    *)
   Definition wp_revert_identity (cls : globname) (Q : mpred) : Rep :=
-    identitiesR true cls [cls] 1 **
-    (identitiesR false cls [] 1 -* pureR Q).
+    identitiesR true cls [cls] (cQp.mut 1) **
+    (identitiesR false cls [] (cQp.mut 1) -* pureR Q).
 
   Theorem wp_revert_identity_frame cls Q Q' :
     pureR (Q' -* Q) |-- wp_revert_identity cls Q' -* wp_revert_identity cls Q.
@@ -118,7 +119,7 @@ Section with_cpp.
 
   (** sanity chect that initialization and revert are inverses *)
   Corollary wp_init_revert cls Q p :
-    let REQ := identitiesR false cls [] 1 in
+    let REQ := identitiesR false cls [] (cQp.mut 1) in
         p |-> REQ ** Q
     |-- p |-> wp_init_identity cls (p |-> wp_revert_identity cls (p |-> REQ ** Q)).
   Proof.
@@ -129,32 +130,65 @@ Section with_cpp.
 
   (** * Binding parameters *)
 
+  Fixpoint wp_make_mutables (ls : list (ptr * type)) (Q : epred) : mpred :=
+    match ls with
+    | nil => Q
+    | (p,t) :: ls => wp_make_mutables ls $ wp_make_mutable tu p t Q
+    end.
+
+  Lemma wp_make_mutables_frame ls : forall Q Q',
+      Q -* Q' |-- wp_make_mutables ls Q -* wp_make_mutables ls Q'.
+  Proof.
+    induction ls =>/=; eauto.
+    iIntros (??) "X"; case_match; iApply (IHls with "[X]").
+    iApply wp_const_frame; first reflexivity; eauto.
+  Qed.
+
+  Definition Kcleanup (ls : list (ptr * type)) : Kpred -> Kpred :=
+    Kat_exit (wp_make_mutables ls).
+
+  Lemma Kcleanup_frame ls (Q Q' : Kpred) rt :
+    Q rt -* Q' rt |-- Kcleanup ls Q rt -* Kcleanup ls Q' rt.
+  Proof.
+    iIntros "K". iApply Kat_exit_frame; eauto.
+    iIntros (??) "X"; iApply wp_make_mutables_frame; eauto.
+  Qed.
+
   (** [bind_vars args vals r Q] preforms initialization of the parameters
       given the values being passed.
+
+      NOTE. We make arguments [const] here if necessary and then make them
+            mutable again in the second argument to [Q].
    *)
   Fixpoint bind_vars (args : list (ident * type)) (ar : function_arity) (ptrs : list ptr)
-    (ρ : option ptr -> region) (Q : region -> FreeTemps -> mpred) : mpred :=
+    (ρ : option ptr -> region) (Q : region -> list (ptr * type) -> mpred) : mpred :=
     match args with
     | nil =>
         match ar with
         | Ar_Definite =>
             match ptrs with
-            | nil => Q (ρ None) FreeTemps.id
+            | nil => Q (ρ None) []
             | _ :: _ => ERROR "bind_vars: extra arguments"
             end
         | Ar_Variadic =>
             match ptrs with
-            | vap :: nil => Q (ρ $ Some vap) FreeTemps.id
+            | vap :: nil => Q (ρ $ Some vap) []
             | _ => ERROR "bind_vars: variadic function missing varargs"
             end
         end
-    | (x,_) :: xs =>
+    | (x,ty) :: xs =>
         match ptrs with
         | p :: ps  =>
-            bind_vars xs ar ps (fun vap => Rbind x p $ ρ vap) Q
+            let '(cv, ty) := decompose_type ty in
+            if q_const cv then
+              wp_make_const tu p ty $ bind_vars xs ar ps (fun vap => Rbind x p $ ρ vap)
+                (fun ρ consts => Q ρ $ (p,ty) :: consts)
+            else
+              bind_vars xs ar ps (fun vap => Rbind x p $ ρ vap) Q
         | nil => ERROR "bind_vars: insufficient arguments"
         end
     end.
+
 
   Lemma bind_vars_frame : forall ts ar args ρ Q Q',
         Forall ρ free, Q ρ free -* Q' ρ free
@@ -163,10 +197,13 @@ Section with_cpp.
     induction ts; destruct args => /= *; eauto.
     { case_match; eauto.
       iIntros "A B"; iApply "A"; eauto. }
-    { case_match; eauto.  case_match; eauto.
+    { case_match; eauto. case_match; eauto.
       iIntros "A"; iApply "A". }
-    { iIntros "A B". destruct a.
-      iRevert "B"; by iApply IHts. }
+    { iIntros "A".
+      repeat case_match; subst.
+      { iApply wp_const_frame; first reflexivity.
+        iApply IHts. iIntros (??). iApply "A". }
+      { iApply IHts; iApply "A". } }
   Qed.
 
   (** * Weakest preconditions of the flavors of C++ "functions"  *)
@@ -179,8 +216,8 @@ Section with_cpp.
       match body with
       | Impl body =>
         let ρ va := Remp None va f.(f_return) in
-        bind_vars f.(f_params) f.(f_arity) args ρ (fun ρ frees =>
-        |> wp ρ body (Kfree frees $ Kreturn (funI x => |={⊤}=> |> Q x)))
+        bind_vars f.(f_params) f.(f_arity) args ρ (fun ρ cleanup =>
+        |> wp ρ body (Kcleanup cleanup $ Kreturn (funI x => |={⊤}=> |> Q x)))
       | Builtin builtin =>
         wp_builtin_func builtin (Tfunction (cc:=f.(f_cc)) f.(f_return) (List.map snd f.(f_params))) args Q
       end
@@ -206,8 +243,8 @@ Section with_cpp.
       match args with
       | thisp :: rest_vals =>
         let ρ va := Remp (Some thisp) va m.(m_return) in
-        bind_vars m.(m_params) m.(m_arity) rest_vals ρ (fun ρ frees =>
-        |> wp ρ body (Kfree frees (Kreturn (funI x => |={⊤}=> |>Q x))))
+        bind_vars m.(m_params) m.(m_arity) rest_vals ρ (fun ρ cleanup =>
+        |> wp ρ body (Kcleanup cleanup (Kreturn (funI x => |={⊤}=> |>Q x))))
       | _ => False
       end
     | Some _ => UNSUPPORTED "defaulted methods"%bs
@@ -335,9 +372,9 @@ Section with_cpp.
       let members := wpi_members ρ cls this s.(s_fields) inits in
       let ident Q := this |-> wp_init_identity cls Q in
       (** initialize the bases, then the identity, then the members *)
-      bases (ident (members (this |-> struct_paddingR 1 cls -*  Q)))
+      bases (ident (members (this |-> struct_paddingR (cQp.mut 1) cls -*  Q)))
       (* NOTE we get the [struct_paddingR] at the end since
-         [struct_paddingR 1 cls |-- type_ptrR (Tnamed cls)].
+         [struct_paddingR (cQp.mut 1) cls |-- type_ptrR (Tnamed cls)].
        *)
     end.
 
@@ -449,25 +486,25 @@ Section with_cpp.
         match tu !! ctor.(c_class) with
         | Some (Gstruct cls) =>
           (* this is a structure *)
-          thisp |-> tblockR ty 1 **
+          thisp |-> tblockR ty (cQp.mut 1) **
           (* ^ this requires that you give up the *entire* block of memory that the object
              will use.
            *)
           |> let ρ va := Remp (Some thisp) va Tvoid in
-             bind_vars ctor.(c_params) ctor.(c_arity) rest_vals ρ (fun ρ frees =>
+             bind_vars ctor.(c_params) ctor.(c_arity) rest_vals ρ (fun ρ cleanup =>
                (wp_struct_initializer_list cls ρ ctor.(c_class) thisp inits
-                  (wp ρ body (Kfree frees (Kreturn_void (|={⊤}=> |> Forall p : ptr, p |-> primR Tvoid 1 Vvoid -* Q p))))))
+                  (wp ρ body (Kcleanup cleanup (Kreturn_void (|={⊤}=> |> Forall p : ptr, p |-> primR Tvoid (cQp.mut 1) Vvoid -* Q p))))))
         | Some (Gunion union) =>
         (* this is a union *)
-          thisp |-> tblockR ty 1 **
+          thisp |-> tblockR ty (cQp.mut 1) **
           (* ^ this requires that you give up the *entire* block of memory that the object
              will use.
            *)
           |> let ρ va := Remp (Some thisp) va Tvoid in
-             bind_vars ctor.(c_params) ctor.(c_arity) rest_vals ρ (fun ρ frees =>
+             bind_vars ctor.(c_params) ctor.(c_arity) rest_vals ρ (fun ρ cleanup =>
                (wp_union_initializer_list union ρ ctor.(c_class) thisp inits
-                  (fun which => wp ρ body (Kfree frees (Kreturn_void (thisp |-> union_paddingR 1 ctor.(c_class) which -*
-                                                                       |={⊤}=> |> Forall p, p |-> primR Tvoid 1 Vvoid -* Q p))))))
+                  (fun which => wp ρ body (Kcleanup cleanup (Kreturn_void (thisp |-> union_paddingR (cQp.mut 1) ctor.(c_class) which -*
+                                                                       |={⊤}=> |> Forall p, p |-> primR Tvoid (cQp.mut 1) Vvoid -* Q p))))))
         | Some _ =>
           ERROR $ "constructor for non-aggregate (" ++ ctor.(c_class) ++ ")"
         | None => False
@@ -486,7 +523,7 @@ Section with_cpp.
   (** ** Weakest precondition of a destructor *)
   Definition wpd_bases (cls : globname) (this : ptr) (bases : list globname) : epred -> mpred :=
     let del_base base := FreeTemps.delete (Tnamed base) (this ,, _base cls base) in
-    interp (FreeTemps.seqsR (List.map del_base bases)).
+    interp (FreeTemps.seqs_rev (List.map del_base bases)).
 
   Lemma wpd_bases_frame cls this : forall bases Q Q',
       Q -* Q' |-- wpd_bases cls this bases Q -* wpd_bases cls this bases Q'.
@@ -494,7 +531,7 @@ Section with_cpp.
 
   Definition wpd_members (cls : globname) (this : ptr) (members : list Member) : epred -> mpred :=
     let del_member m := FreeTemps.delete m.(mem_type) (this ,, _field {| f_name := m.(mem_name) ; f_type := cls |}) in
-    interp (FreeTemps.seqsR (List.map del_member members)).
+    interp (FreeTemps.seqs_rev (List.map del_member members)).
 
   Lemma wpd_members_frame cls this : forall members Q Q',
       Q -* Q' |-- wpd_members cls this members Q -* wpd_members cls this members Q'.
@@ -520,14 +557,14 @@ Section with_cpp.
       let epilog :=
           match tu !! dtor.(d_class) with
           | Some (Gstruct s) => Some $ fun (thisp : ptr) =>
-            thisp |-> struct_paddingR 1 dtor.(d_class) **
+            thisp |-> struct_paddingR (cQp.mut 1) dtor.(d_class) **
             wpd_members dtor.(d_class) thisp s.(s_fields)
                (* ^ fields are destroyed *)
                (thisp |-> wp_revert_identity dtor.(d_class)
                (* ^ the identity of the object is destroyed *)
                   (wpd_bases dtor.(d_class) thisp (List.map fst s.(s_bases))
                   (* ^ the base classes are destroyed (reverse order) *)
-                     (thisp |-> tblockR (Tnamed dtor.(d_class)) 1 -* |={⊤}=> |> Forall p : ptr, p |-> primR Tvoid 1 Vvoid -* Q p)))
+                     (thisp |-> tblockR (Tnamed dtor.(d_class)) (cQp.mut 1) -* |={⊤}=> |> Forall p : ptr, p |-> primR Tvoid (cQp.mut 1) Vvoid -* Q p)))
                      (* ^ the operations above destroy each object returning its memory to
                         the abstract machine. Then the abstract machine gives this memory
                         back to the program.
@@ -542,8 +579,8 @@ Section with_cpp.
                automatically where they can prove the active entry has a trivial destructor
                or is already destroyed.
              *)
-            |={⊤}=> thisp |-> tblockR (Tnamed dtor.(d_class)) 1 **
-                   (thisp |-> tblockR (Tnamed dtor.(d_class)) 1 -* |={⊤}=> |> Forall p : ptr, p |-> primR Tvoid 1 Vvoid -* Q p)
+            |={⊤}=> thisp |-> tblockR (Tnamed dtor.(d_class)) (cQp.mut 1) **
+                   (thisp |-> tblockR (Tnamed dtor.(d_class)) (cQp.mut 1) -* |={⊤}=> |> Forall p : ptr, p |-> primR Tvoid (cQp.mut 1) Vvoid -* Q p)
           | _ => None
           end%I
       in
