theories/lang/cpp/logic/new_delete.v
@@ -76,7 +76,7 @@ Module Type Expr__newdelete.
       #[local] Notation Tbyte := Tuchar (only parsing).
 
       Definition alloc_size_t (sz : N) (Q : ptr -> (mpred -> mpred) -> mpred) : mpred :=
-        Forall p : ptr, p |-> primR Tsize_t 1 (Vn sz) -* Q p (fun Q => p |-> anyR Tsize_t 1 ** Q).
+        Forall p : ptr, p |-> primR Tsize_t (cQp.mut 1) (Vn sz) -* Q p (fun Q => p |-> anyR Tsize_t (cQp.mut 1) ** Q).
 
       Section new.
         (** [new (...) C(...)] <https://eel.is/c++draft/expr.new>
@@ -132,12 +132,12 @@ Module Type Expr__newdelete.
                 Exists sz al, [| size_of aty = Some sz |] ** [| has_type sz Tsize_t |] ** [| align_of aty = Some al |] **
                 Reduce (alloc_size_t sz (fun p FR =>
                 |> fspec tu.(globals) nfty (_global new_fn.1) (p :: vs) (fun res => FR $
-                      Exists storage_ptr : ptr, res |-> primR (Tptr Tvoid) 1 (Vptr storage_ptr) **
+                      Exists storage_ptr : ptr, res |-> primR (Tptr Tvoid) (cQp.mut 1) (Vptr storage_ptr) **
                         if bool_decide (storage_ptr = nullptr) then
                           [| new_args <> nil |] ** Q (Vptr storage_ptr) free
                         else
                           (* [blockR sz -|- tblockR aty] *)
-                          (storage_ptr |-> (blockR sz 1 ** alignedR al) **
+                          (storage_ptr |-> (blockR sz (cQp.m 1) ** alignedR al) **
                            (* TODO: ^ This misses an condition that [storage_ptr]
                               is suitably aligned, accounting for
                               __STDCPP_DEFAULT_NEW_ALIGNMENT__ (issue #149) *)
@@ -148,20 +148,22 @@ Module Type Expr__newdelete.
                                   match oinit with
                                   | None => (* default_initialize the memory *)
                                     default_initialize aty obj_ptr
-                                                       (fun free' =>
-                                                          (* Track the type we are allocating
-                                                             so it can be checked at [delete]
-                                                           *)
-                                                          obj_ptr |-> new_tokenR 1 aty -*
-                                                          Q (Vptr obj_ptr) (free' >*> free))
+                                      (fun free' =>
+                                         (* Track the type we are allocating
+                                            so it can be checked at [delete].
+                                            It is important that this preseves
+                                            `const`ness of the type.
+                                          *)
+                                         obj_ptr |-> new_tokenR (cQp.mut 1) aty -*
+                                         Q (Vptr obj_ptr) (free' >*> free))
                                   | Some init => (* Use [init] to initialize the memory *)
                                     wp_initialize aty obj_ptr init
-                                            (fun free' =>
-                                               (* Track the type we are allocating
-                                                  so it can be checked at [delete]
-                                                *)
-                                               obj_ptr |-> new_tokenR 1 aty -*
-                                               Q (Vptr obj_ptr) (free' >*> free))
+                                      (fun free' =>
+                                         (* Track the type we are allocating
+                                            so it can be checked at [delete]
+                                          *)
+                                         obj_ptr |-> new_tokenR (cQp.mut 1) aty -*
+                                         Q (Vptr obj_ptr) (free' >*> free))
                                   end))))))
         |-- wp_operand (Enew new_fn new_args aty None oinit) Q.
 
@@ -205,12 +207,12 @@ Module Type Expr__newdelete.
                     Forall sz',
                       Reduce (alloc_size_t (sz' + sz) (fun psz FR =>
                       |> fspec tu.(globals) nfty (_global new_fn.1) (psz :: vs) (fun res => FR $
-                        Exists storage_ptr : ptr, res |-> primR (Tptr Tvoid) 1 (Vptr storage_ptr) **
+                        Exists storage_ptr : ptr, res |-> primR (Tptr Tvoid) (cQp.mut 1) (Vptr storage_ptr) **
                           if bool_decide (storage_ptr = nullptr) then
                             [| new_args <> nil |] ** Q (Vptr storage_ptr) free
                           else
                             (* [blockR sz -|- tblockR (Tarray aty array_size)] *)
-                            (storage_ptr |-> blockR (sz' + sz) 1 **
+                            (storage_ptr |-> blockR (sz' + sz) (cQp.m 1) **
                              storage_ptr .[Tu8 ! sz'] |-> alignedR al) **
                              (* todo: ^ This misses an condition that [storage_ptr]
                               is suitably aligned, accounting for
@@ -218,9 +220,7 @@ Module Type Expr__newdelete.
                                 (Forall obj_ptr : ptr,
                                    (* This also ensures these pointers share their
                                    address (see [provides_storage_same_address]) *)
-                                   provides_storage
-                                     (storage_ptr .[Tu8 ! sz'])
-                                     obj_ptr array_ty -*
+                                   provides_storage (storage_ptr .[Tu8 ! sz']) obj_ptr array_ty -*
                                    match oinit with
                                    | None => (* default_initialize the memory *)
                                      default_initialize array_ty obj_ptr
@@ -228,7 +228,7 @@ Module Type Expr__newdelete.
                                                            (* Track the type we are allocating
                                                               so it can be checked at [delete]
                                                             *)
-                                                           obj_ptr |-> new_tokenR 1 array_ty -*
+                                                           obj_ptr |-> new_tokenR (cQp.mut 1) array_ty -*
                                                            Q (Vptr obj_ptr)
                                                              (free'' >*> free' >*> free))
                                    | Some init => (* Use [init] to initialize the memory *)
@@ -237,7 +237,7 @@ Module Type Expr__newdelete.
                                                       (* Track the type we are allocating
                                                          so it can be checked at [delete]
                                                        *)
-                                                      obj_ptr |-> new_tokenR 1 array_ty -*
+                                                      obj_ptr |-> new_tokenR (cQp.mut 1) array_ty -*
                                                       Q (Vptr obj_ptr)
                                                         (free'' >*> free' >*> free))
                                    end))))))
@@ -246,7 +246,7 @@ Module Type Expr__newdelete.
 
       Section delete.
         Definition alloc_pointer (pv : ptr) (Q : ptr -> FreeTemp -> mpred) : mpred :=
-          Forall p : ptr, p |-> primR (Tptr Tvoid) 1 (Vptr pv) -* Q p (FreeTemps.delete (Tptr Tvoid) p).
+          Forall p : ptr, p |-> primR (Tptr Tvoid) (cQp.mut 1) (Vptr pv) -* Q p (FreeTemps.delete (Tptr Tvoid) p).
 
         Lemma alloc_pointer_frame : forall p Q Q',
             Forall p fr, Q p fr -* Q' p fr |-- alloc_pointer p Q -* alloc_pointer p Q'.
@@ -324,6 +324,8 @@ Module Type Expr__newdelete.
           iApply resolve_virtual_frame. iIntros (???); iApply "X".
         Qed.
 
+        Definition cv_compat (t1 t2 : type) : Prop :=
+          erase_qualifiers t1 = erase_qualifiers t2.
 
         (* delete
 
@@ -364,7 +366,8 @@ Module Type Expr__newdelete.
              else
                (* v---- Calling destructor with object pointer *)
                resolve_dtor destroyed_type obj_ptr (fun this' mdc_ty =>
-                    this' |-> new_tokenR 1 mdc_ty **
+                    Exists cv_mdc, this' |-> new_tokenR (cQp.mut 1) cv_mdc **
+                                   [| cv_compat cv_mdc mdc_ty |] **
                     (* v---- because dispatch could be virtual, the translation unit
                              used to destroy the object may need to be different *)
                     Exists tu', denoteModule tu' ** destroy_val tu' mdc_ty this' (
@@ -374,7 +377,7 @@ Module Type Expr__newdelete.
                       (* Transfer memory to underlying storage pointer; unlike in
                          [end_provides_storage], this memory was pre-destructed by
                          [delete_val]. *)
-                      (storage_ptr |-> blockR sz 1 -*
+                      (storage_ptr |-> blockR sz (cQp.m 1) -*
                        (* v---- Calling deallocator with storage pointer
                                 Like above, because the operation is on the MDC,
                                 we must use [tu'] *)
@@ -401,7 +404,7 @@ Module Type Expr__newdelete.
                let array_ty := Tarray destroyed_type array_size in
                (* /---- Token for distinguishing between array and
                   v     non-array allocations *)
-               obj_ptr |-> new_tokenR 1 array_ty **
+               obj_ptr |-> new_tokenR (cQp.mut 1) array_ty **
                (* /---- Calling destructor with object pointer
                   v     Note: virtual dispatch is not allowed for [delete[]] *)
                destroy_val tu array_ty obj_ptr (
@@ -414,7 +417,7 @@ Module Type Expr__newdelete.
                       (* Transfer memory to underlying storage pointer; unlike in
                          [end_provides_storage], this memory was pre-destructed by
                          [delete_val]. *)
-                      (storage_ptr |-> blockR (sz' + sz) 1 -*
+                      (storage_ptr |-> blockR (sz' + sz) (cQp.m 1) -*
                        (* v---- Calling deallocator with storage pointer.
                           Note: we rely on the AST to have correctly resolved this since the dispatch is statically known.
                         *)
